Cumulative updates

src/CCSLib.sig
@@ -7,11 +7,8 @@ signature CCSLib =
 sig
   include Abbrev
 
-  val PAT_X_ASSUM               : term -> thm_tactic -> tactic
-  val qpat_x_assum              : Q.tmquote -> thm_tactic -> tactic
-  val Q_GENL                    : Q.tmquote list -> thm -> thm
   val fix                       : Q.tmquote list -> tactic
-  val set                       : Q.tmquote list -> tactic
+  val unset                     : Q.tmquote list -> tactic
   val take                      : Q.tmquote list -> tactic
   val Know                      : Q.tmquote -> tactic
   val Suff                      : Q.tmquote -> tactic
@@ -25,7 +22,7 @@ sig
   val PRINT_TAC                 : string -> tactic
   val COUNT_TAC                 : tactic -> tactic
   val STRONG_CONJ_TAC           : tactic
-  val X_TAC                     : int -> tactic
+  val NDISJ_TAC                 : int -> tactic
 
   val ONCE_REWRITE_RHS_RULE     : thm list -> thm -> thm
   val PURE_REWRITE_RHS_RULE     : thm list -> thm -> thm
